Co-inductive tower

theories/Testing_Pre_orders/Must/Alternative_Preorder/Co_Inductive_Tower_Acceptance_Set/Coin_tower.v
@@ -40,97 +40,111 @@ From TestingTheory Require Import
 
 (* TODO: define me using the coinduction library *)
 
-Section copre.
-  Context `{@FiniteImagegLts P A H gLtsP, @FiniteImagegLts Q A H gLtsQ}.
-  Context `{gLtsT : !gLtsEq T H}.
-  Context `{@AbsAction P T FinA PreAct A H Φ 𝝳P _ _ }.
-  Context `{@AbsAction Q T FinA PreAct A H Φ 𝝳Q _ _ }.
+Record copre_ `{@FiniteImagegLts P A H gLtsP, @FiniteImagegLts Q A H gLtsQ}
+  `{gLtsT : !gLtsEq T H}
+  `{@AbsAction P T FinA PreAct A H Φ 𝝳P _ _ }
+  `{@AbsAction Q T FinA PreAct A H Φ 𝝳Q _ _ }
+  (FIX : gset P -> gset Q -> Prop) (X : gset P) (Y : gset Q) : Prop := {
+    c_tau_ Y' : wt_set_from_pset_spec1 Y [] Y' -> FIX X Y'
+  ; c_now_ : X ⤓ -> forall q , q ∈ Y -> q ↛ ->
+            exists p, p ∈ X /\ exists p', p ⟹ p' /\ p' ↛ /\ ⌈ (𝝳P ∘ Φ) ⌉ (coR p') ⊆ ⌈ (𝝳Q ∘ Φ) ⌉ (coR q)
+  ; c_step_ : forall μ Y' X', X ⇓ [μ] ->
+                         wt_set_from_pset_spec1 Y [μ] Y' -> wt_set_from_pset_spec X [μ] X' -> FIX X' Y'
+  ; c_cnv_ : X ⤓ -> Y ⤓
+  }. Check c_tau_.
+  #[global] Arguments c_tau_ {_ _ _ _ _ _ _ _ _ _ _ _ _ _ _ _ _ FIX X Y}.
+  #[global] Arguments c_now_ {_ _ _ _ _ _ _ _ _ _ _ _ _ _ _ _ _ FIX X Y}.
+  #[global] Arguments c_step_ {_ _ _ _ _ _ _ _ _ _ _ _ _ _ _ _ _ FIX X Y}.
+  #[global] Arguments c_cnv_ {_ _ _ _ _ _ _ _ _ _ _ _ _ _ _ _ _ FIX X Y}.
 
-  Definition REL := gset P -> gset Q -> Prop.
-
-  Record copre_ (FIX : REL) (ps : gset P) (qs : gset Q) : Prop := {
-    c_tau_ qs' : wt_set_from_pset_spec1 qs [] qs' -> FIX ps qs'
-  ; c_now_ : ps ⤓ -> forall q , q ∈ qs -> q ↛ ->
-            exists p, p ∈ ps /\ exists p', p ⟹ p' /\ p' ↛ /\ ⌈ (𝝳P ∘ Φ) ⌉ (coR p') ⊆ ⌈ (𝝳Q ∘ Φ) ⌉ (coR q)
-  ; c_step_ : forall μ qs' ps', ps ⇓ [μ] ->
-                         wt_set_from_pset_spec1 qs [μ] qs' -> wt_set_from_pset_spec ps [μ] ps' -> FIX ps' qs'
-  ; c_cnv_ : ps ⤓ -> qs ⤓
-  }.
-  #[global] Arguments c_tau_ {FIX ps qs}.
-  #[global] Arguments c_now_ {FIX ps qs}.
-  #[global] Arguments c_step_ {FIX ps qs}.
-  #[global] Arguments c_cnv_ {FIX ps qs}.
-
-  Program Definition copre_m : mon REL := {| body := copre_ |} .
+  Program Definition copre_m 
+  `{@FiniteImagegLts P A H gLtsP, @FiniteImagegLts Q A H gLtsQ}
+  `{gLtsT : !gLtsEq T H}
+  `{AbsPT : @AbsAction P T FinA PreAct A H Φ 𝝳P _ _ }
+  `{AbsQT : @AbsAction Q T FinA PreAct A H Φ 𝝳Q _ _ } : mon (gset P -> gset Q -> Prop) := 
+  {| body := (@copre_ P A H _ _ Q _ _ T _ _ _ Φ 𝝳P AbsPT 𝝳Q AbsQT) |} .
   Next Obligation.
-    intros F1 F2 HF ps qs h; constructor.
+    intros F1 F2 HF X Y h; constructor.
     - intros; apply HF, h.(c_tau_); auto.
     - exact h.(c_now_).
     - intros; eapply HF, h.(c_step_); auto.
+      + exact H2.
+      + exact H3.
       + exact H4.
-      + exact H5.
-      + exact H6.
     - exact h.(c_cnv_).
   Qed.
 
-  Definition copre := gfp copre_m .
+  Definition copre `{@FiniteImagegLts P A H gLtsP, @FiniteImagegLts Q A H gLtsQ}
+  `{gLtsT : !gLtsEq T H}
+  `{AbsPT : @AbsAction P T FinA PreAct A H Φ 𝝳P _ _ }
+  `{AbsQT : @AbsAction Q T FinA PreAct A H Φ 𝝳Q _ _ } := 
+  gfp (@copre_m P A H _ _ Q _ _ T _ _ _ Φ 𝝳P AbsPT 𝝳Q AbsQT).
 
-  Notation "ps ⩽ₜₒᵥᵥₑᵣ qs" := (copre ps qs) (at level 70).
+  Notation "X ⩽ₜₒᵥᵥₑᵣ Y" := (copre X Y) (at level 70).
 
-  Lemma c_tau {ps qs qs'} : ps ⩽ₜₒᵥᵥₑᵣ qs -> wt_set_from_pset_spec1 qs [] qs' -> ps ⩽ₜₒᵥᵥₑᵣ qs' .
+Section copre.
+  Context `{@FiniteImagegLts P A H gLtsP, @FiniteImagegLts Q A H gLtsQ}.
+  Context `{gLtsT : !gLtsEq T H}.
+  Context `{AbsPT : @AbsAction P T FinA PreAct A H Φ 𝝳P _ _ }.
+  Context `{AbsQT : @AbsAction Q T FinA PreAct A H Φ 𝝳Q _ _ }.
+
+  Definition REL := gset P -> gset Q -> Prop.
+
+  Lemma c_tau {X : gset P } { Y Y' : gset Q} : X ⩽ₜₒᵥᵥₑᵣ Y -> wt_set_from_pset_spec1 Y [] Y' -> X ⩽ₜₒᵥᵥₑᵣ Y' .
   Proof.
-    intros h%(gfp_pfp copre_m); intros; now apply h.(c_tau_).
+    intros h%(gfp_pfp copre_m) ; intros; now apply h.(c_tau_).
   Qed.
 
-  Lemma c_tau' {PRE : Chain copre_m} {ps qs qs'} :
-    copre_m (elem PRE) ps qs -> wt_set_from_pset_spec1 qs [] qs' -> elem PRE ps qs' .
+  Lemma c_tau' {PRE : Chain (@copre_m P A H _ _ Q _ _ T _ _ _ Φ 𝝳P AbsPT 𝝳Q AbsQT)} { X : gset P } { Y Y' : gset Q} :
+    (@copre_m P A H _ _ Q _ _ T _ _ _ Φ 𝝳P AbsPT 𝝳Q AbsQT) (elem PRE) X Y -> wt_set_from_pset_spec1 Y [] Y' -> elem PRE X Y' .
   Proof.
     intros h Ht. now apply h.(c_tau_). Qed.
 
-  Lemma c_now {ps qs}
-    : ps ⩽ₜₒᵥᵥₑᵣ qs
-      -> ps ⤓
-      -> forall q , q ∈ qs -> q ↛
-      -> exists p, p ∈ ps
+  Lemma c_now { X : gset P } { Y : gset Q}
+    : X ⩽ₜₒᵥᵥₑᵣ Y
+      -> X ⤓
+      -> forall q , q ∈ Y -> q ↛
+      -> exists p, p ∈ X
                 /\ exists p', p ⟹ p'
                 /\ p' ↛
                 /\ ⌈ (𝝳P ∘ Φ) ⌉ (coR p') ⊆ ⌈ (𝝳Q ∘ Φ) ⌉ (coR q) .
   Proof.
-    intros h%(gfp_pfp copre_m); intros; now apply h.(c_now_).
+    intros h%(gfp_pfp copre_m); intros.
+    eapply h.(c_now_);eauto.
   Qed.
 
-  Lemma c_step {ps ps' qs qs' μ}
-    : ps ⩽ₜₒᵥᵥₑᵣ qs
-      -> ps ⇓ [μ]
-      -> wt_set_from_pset_spec1 qs [μ] qs'
-      -> wt_set_from_pset_spec ps [μ] ps'
-      -> ps' ⩽ₜₒᵥᵥₑᵣ qs' .
+  Lemma c_step { X X' : gset P } { Y Y' : gset Q} {μ}
+    : X ⩽ₜₒᵥᵥₑᵣ Y
+      -> X ⇓ [μ]
+      -> wt_set_from_pset_spec1 Y [μ] Y'
+      -> wt_set_from_pset_spec X [μ] X'
+      -> X' ⩽ₜₒᵥᵥₑᵣ Y' .
   Proof.
     intros h%(gfp_pfp copre_m); intros; now eapply h.(c_step_); eauto.
   Qed.
 
-  Lemma c_cnv {ps qs}
-    : ps ⩽ₜₒᵥᵥₑᵣ qs
-      -> ps ⤓
-      -> qs ⤓ .
+  Lemma c_cnv { X : gset P } { Y : gset Q}
+    : X ⩽ₜₒᵥᵥₑᵣ Y
+      -> X ⤓
+      -> Y ⤓ .
   Proof.
     intros h%(gfp_pfp copre_m); intros; now eapply h.(c_cnv_); eauto.
   Qed.
 
-  Lemma copre_if_prex (ps : gset P) (qs : gset Q) : ps ≼ₛₑₜ_ₐₛ qs -> ps ⩽ₜₒᵥᵥₑᵣ qs.
+  Lemma copre_if_prex (X : gset P) (Y : gset Q) : X ≼ₛₑₜ_ₐₛ Y -> X ⩽ₜₒᵥᵥₑᵣ Y.
   Proof.
-    revert ps qs; unfold copre.
+    revert X Y; unfold copre.
     coinduction RR CIH.
-    intros ps qs (hsub1 & hsub2).
+    intros X Y (hsub1 & hsub2).
     constructor.
-    - intros qs' l.
+    - intros Y' l.
       eapply CIH, bhvx_preserved_by_reductions; eauto. split; eauto.
     - intros hterm q mem hst.
       destruct (hsub2 q [] q mem) as (p' & hw & hstp' & hsub0); eauto.
       + eapply wt_nil.
       + intros p' mem'; constructor.
         eapply termination_if_termination_set_helper;eauto.
-    - intros μ qs' ps' hcnv hw wtspec.
+    - intros μ Y' ps' hcnv hw wtspec.
       eapply CIH, bhvx_preserved_by_external_action; eauto.
       + inversion hcnv;subst. eapply termination_if_termination_set_helper;eauto.
       + split;eauto.
@@ -141,24 +155,24 @@ Section copre.
   Qed.
 
   Lemma co_preserved_by_wt_nil
-    (ps : gset P) (qs qs' : gset Q) : wt_set_from_pset_spec1 qs [] qs' -> ps ⩽ₜₒᵥᵥₑᵣ qs -> ps ⩽ₜₒᵥᵥₑᵣ qs'.
+    (X : gset P) (Y Y' : gset Q) : wt_set_from_pset_spec1 Y [] Y' -> X ⩽ₜₒᵥᵥₑᵣ Y -> X ⩽ₜₒᵥᵥₑᵣ Y'.
   Proof.
     intros hw Hyp. eapply c_tau;eauto.
   Qed.
 
 
-  Lemma prex1_if_copre (ps : gset P) (qs : gset Q) : ps ⩽ₜₒᵥᵥₑᵣ qs -> ps ₁≼ₛₑₜ_ₐₛ qs.
+  Lemma prex1_if_copre (X : gset P) (Y : gset Q) : X ⩽ₜₒᵥᵥₑᵣ Y -> X ₁≼ₛₑₜ_ₐₛ Y.
   Proof.
-    intros hpq s; revert ps qs hpq.
-    dependent induction s; intros ps qs hpq hcnv.
+    intros hpq s; revert X Y hpq.
+    dependent induction s; intros X Y hpq hcnv.
     + eapply convergence_set_if_convergence_forall in hcnv.
       eapply convergence_forall_if_convergence_set.
       eapply equiv_termination. eapply (c_cnv hpq).
       eapply equiv_termination. exact hcnv.
-    + assert (qs ⤓).
+    + assert (Y ⤓).
       { eapply convergence_set_if_convergence_forall in hcnv. inversion hcnv; subst.
       eapply (c_cnv hpq). eauto. }
-      assert (hcnv0 : ∀ p : P, p ∈ ps → p ⇓ [a]) by (intros; now eapply cnv_wk, hcnv).
+      assert (hcnv0 : ∀ p : P, p ∈ X → p ⇓ [a]) by (intros; now eapply cnv_wk, hcnv).
       intros. eapply cnv_act; eauto. eapply termination_if_termination_set_helper;eauto.
       intros q' hw.
       eapply IHs.
@@ -167,18 +181,18 @@ Section copre.
          * intros q'' mem. exists q. split;eauto.
            instantiate (1:= {[ q' ]}) in mem.
            assert (q'' = q') by set_solver. subst. exact hw.
-         * eapply (wt_s_set_from_pset_ispec ps [a] hcnv0); eauto.
+         * eapply (wt_s_set_from_pset_ispec X [a] hcnv0); eauto.
       ++ intros p mem.
-         edestruct (wt_s_set_from_pset_ispec ps [a] hcnv0) as (TrSet_hyp1 & TrSet_hyp2).
+         edestruct (wt_s_set_from_pset_ispec X [a] hcnv0) as (TrSet_hyp1 & TrSet_hyp2).
          eapply TrSet_hyp1 in mem as (p0 & hmem0%hcnv & hw0).
          inversion hmem0; subst. eauto.
       ++ set_solver.
   Qed.
 
-  Lemma prex2_if_copre (ps : gset P) (qs : gset Q) : ps ⩽ₜₒᵥᵥₑᵣ qs -> ps ₂≼ₛₑₜ_ₐₛ qs.
+  Lemma prex2_if_copre (X : gset P) (Y : gset Q) : X ⩽ₜₒᵥᵥₑᵣ Y -> X ₂≼ₛₑₜ_ₐₛ Y.
   Proof.
-    intros hsub q s q' mem; revert ps qs q q' mem hsub ; dependent induction s; intros ps qs q q' mem hsub.
-    + intros hw hstq' hcnv. revert ps qs mem hsub hstq' hcnv.
+    intros hsub q s q' mem; revert X Y q q' mem hsub ; dependent induction s; intros X Y q q' mem hsub.
+    + intros hw hstq' hcnv. revert X Y mem hsub hstq' hcnv.
       dependent induction hw;intros.
       * edestruct (c_now hsub).
         - eapply equiv_termination.
@@ -198,33 +212,33 @@ Section copre.
       change (μ :: s) with ([μ] ++ s) in hqq'.
       eapply wt_split in hqq' as (q0 & hw0 & hw1).
       eapply wt_decomp_one in hw0 as (q0' & q1' & q1 & hlt & hw0').
-      assert (ps ⩽ₜₒᵥᵥₑᵣ {[ q0' ]}).
+      assert (X ⩽ₜₒᵥᵥₑᵣ {[ q0' ]}).
       { eapply co_preserved_by_wt_nil; eauto. intros q'' mem''.
         assert (q'' = q0') by set_solver. subst. eauto. }
-      assert (hcnv' : ∀ p : P, p ∈ ps → p ⇓ [μ]) by (intros; now eapply cnv_wk, hcnv).
-      assert (∀ p : P, p ∈ ps → p ⇓ [μ]) as hp_conv;eauto.
+      assert (hcnv' : ∀ p : P, p ∈ X → p ⇓ [μ]) by (intros; now eapply cnv_wk, hcnv).
+      assert (∀ p : P, p ∈ X → p ⇓ [μ]) as hp_conv;eauto.
       eapply convergence_set_if_convergence_forall in hp_conv.
-      set (ps' := wt_s_set_from_pset ps [μ] hcnv').
-      assert (ps' ⩽ₜₒᵥᵥₑᵣ {[ q1' ]}) as hpq''. {
+      set (X' := wt_s_set_from_pset X [μ] hcnv').
+      assert (X' ⩽ₜₒᵥᵥₑᵣ {[ q1' ]}) as hpq''. {
         eapply c_step;eauto.
         + intros q''' mem'''. assert (q''' = q1') by set_solver. subst.
           exists q0'. split. set_solver. eapply lts_to_wt;eauto.
         + eapply wt_s_set_from_pset_ispec.
       }
-      assert (ps' ⩽ₜₒᵥᵥₑᵣ {[ q0 ]}) as hp'q.
+      assert (X' ⩽ₜₒᵥᵥₑᵣ {[ q0 ]}) as hp'q.
       { eapply co_preserved_by_wt_nil; eauto. intros q''' mem'''.
         assert (q''' = q0) by set_solver. subst. exists q1'. split;eauto. set_solver.
       }
-      edestruct (IHs ps' ({[ q0 ]})) as (r & memr & p' & hwr & hst & hsub').
+      edestruct (IHs X' ({[ q0 ]})) as (r & memr & p' & hwr & hst & hsub').
       * instantiate (1:= q0). set_solver.
       * eauto.
       * exact hw1.
       * exact hq.
       * intros p hp.
-        edestruct (wt_s_set_from_pset_ispec ps [μ] hcnv') as (TrSet_hyp1 & TrSet_hyp2).
+        edestruct (wt_s_set_from_pset_ispec X [μ] hcnv') as (TrSet_hyp1 & TrSet_hyp2).
         eapply TrSet_hyp1 in hp as (p0 & hmem0 & hw0).
         eapply cnv_preserved_by_wt_act; eauto.
-      * edestruct (wt_s_set_from_pset_ispec ps [μ] hcnv') as (TrSet_hyp1 & TrSet_hyp2).
+      * edestruct (wt_s_set_from_pset_ispec X [μ] hcnv') as (TrSet_hyp1 & TrSet_hyp2).
         eapply TrSet_hyp1 in memr as (p0  & hmem0 & hw0).
         exists p0; split; [ auto | ].
         exists p'; split; [ | split; eauto ].
@@ -239,8 +253,6 @@ Section copre.
     intros hco; split; [ now eapply prex1_if_copre | now eapply prex2_if_copre ].
   Qed.
 End copre.
-
-Notation "X ⩽ₜₒᵥᵥₑᵣ Y" := (copre X Y) (at level 70).
 
 Section eq_contextual.
   Context `{outcome : T -> Prop}.
@@ -271,21 +283,21 @@ Section eq_contextual.
   Context `{!gLtsObaFB P A, !FiniteOutputChain_LtsOba P}.
   Context `{!gLtsObaFB Q A, !FiniteOutputChain_LtsOba Q}.
   Context `{!gLtsObaFB T A, !FiniteOutputChain_LtsOba T}.
-  Check @copre.
+
   Theorem eq_ctx (p : P) (q : Q) :
     pre_extensional outcome p q <-> 
-    (@copre (P * mb A) A _ _ _ (Q * mb A) _ _ _ _ Φ 𝝳 𝝳) ({[ p ▷ (∅ : mb A) ]} : gset (P * mb A))  ({[ q ▷ (∅ : mb A) ]} : gset (Q * mb A)).
+    ({[ p ▷ (∅ : mb A) ]} : gset (P * mb A)) ⩽ₜₒᵥᵥₑᵣ ({[ q ▷ (∅ : mb A) ]} : gset (Q * mb A)).
   Proof.
     rewrite <- eqx. rewrite alt_set_singleton_iff.
     now rewrite equivalence_bhv_acc_ctx.
   Qed.
 End eq_contextual.
 
-(*
-Lemma coin_refl `{@FiniteImagegLts P A H gLtsP}
-  `{CC : Countable PreAct}
-  `{!@FinitaryAbsAction P T FinA PreAct A H Φ 𝝳 _ _ _ _ }
-  {PRE : Chain copre_m} {p : P} : elem PRE {[ p ]} p.
+
+Lemma coin_refl
+  `{@FiniteImagegLts P A H gLtsP}
+  `{gLtsT : !gLtsEq T H} `{AbsPT : @AbsAction P T FinA PreAct A H Φ 𝝳P _ _ }
+  {PRE : Chain copre_m} {p : P} : elem PRE {[ p ]} {[ p ]}.
 Proof.
   apply (gfp_chain PRE).
   eapply eqx.
@@ -293,8 +305,9 @@ Proof.
   firstorder.
 Qed.
 
-Global Instance Proper_elem `{@FiniteImagegLts P A H gLtsP}
-  `{PreAP : @PreExtAction P A H FinA PreA PreA_eq PreA_countable 𝝳 Φ gLtsP}
+Global Instance Proper_elem 
+  `{@FiniteImagegLts P A H gLtsP}
+  `{gLtsT : !gLtsEq T H} `{AbsPT : @AbsAction P T FinA PreAct A H Φ 𝝳P _ _ }
   {PRE : Chain copre_m} :
   Proper ((≡) ==> (=) ==> (iff)) (elem PRE).
 Proof.
@@ -302,17 +315,26 @@ Proof.
   now rewrite (leibniz_equiv _ _ HX).
 Qed.
 
-Global Instance Proper_lts_pre_co_actions `{gLtsOba P A}
-  `{PreAP : @PreExtAction P A H FinA PreA PreA_eq PreA_countable 𝝳 Φ gLtsP}:
-  Proper ((eq_rel) ==> (=)) pre_co_actions_of.
+Global Instance Proper_lts_pre_co_actions `{gLtsEq P A} `{Γ : A -> PreAct}:
+  Proper ((eq_rel) ==> (≡)) (fun p => ⌈ Γ ⌉ (coR p)).
 Proof.
-  intros μ μ' Heq. apply leibniz_equiv.
-  intros x. split.
-  - intro Hyp. admit.
-  - intro Hyp. admit.
-Admitted.
+  intros p p' Heq. intro μ_phi. split.
+  (* apply leibniz_equiv. intros Hyp. split. *)
+  - intro Hyp. destruct Hyp as (μ & mem_coR & eq);subst.
+    destruct mem_coR as (μ' & accepts & duo & b).
+    eapply accepts_preserved_by_eq in accepts;eauto.
+    assert (μ ∈ coR p') as mem.
+    { exists μ'. repeat split; eauto. }
+    eapply map_gamma_of_action;eauto.
+  - intro Hyp. destruct Hyp as (μ & mem_coR & eq);subst.
+    destruct mem_coR as (μ' & accepts & duo & b). symmetry in Heq.
+    eapply accepts_preserved_by_eq in accepts;eauto.
+    assert (μ ∈ coR p) as mem.
+    { exists μ'. repeat split; eauto. }
+    eapply map_gamma_of_action;eauto.
+Qed.
 
-Global Instance Proper_lts_stable `{gLtsOba P A}:
+Global Instance Proper_lts_stable `{gLtsEq P A}:
   Proper ((eq_rel) ==> (=) ==> (impl)) lts_refuses.
 Proof.
   intros p p' Heq α α' ? Hs; subst α'.
@@ -325,8 +347,10 @@ Qed.
 
 (* In the case of a Lts with equivalence relation, the right hand side can also
   be rewritten *)
-Global Instance Proper_eq_rel `{@gLtsOba P A H gLtsEqP} `{!FiniteImagegLts P A}
-  `{PreAP : @PreExtAction P A H FinA PreA PreA_eq PreA_countable 𝝳 Φ _}
+(* Global Instance Proper_eq_rel 
+  `{gLtsP : @gLtsEq P A H}
+  `{!FiniteImagegLts P A} 
+  `{gLtsT : !gLtsEq T H} `{AbsPT : !@AbsAction P T FinA PreAct A H Φ 𝝳P _ _ } 
    {PRE : Chain copre_m}:
   Proper ((≡) ==> (eq_rel) ==> (impl)) (elem PRE).
 Proof.
@@ -347,12 +371,13 @@ Proof.
       * exists y0. split; trivial.
       * eapply Heq; eauto. eapply h.(c_step_) with μ; eauto.
     + intro ht. eapply terminate_preserved_by_eq2; eauto. now apply h.(c_cnv_).
-Qed.
+Qed. *)
 
 Lemma coin_union_l `{@FiniteImagegLts P A H gLtsP}
-  `{PreAP : @PreExtAction P A H FinA PreA PreA_eq PreA_countable 𝝳 Φ gLtsP}
+  `{gLtsT : !gLtsEq T H}
+  `{AbsPT : @AbsAction P T FinA PreAct A H Φ 𝝳P _ _ }
   {PRE : Chain copre_m}
-  : forall (X1 X2 : gset P) (q : P), elem PRE X1 q -> elem PRE (X1 ∪ X2) q.
+  : forall (X1 X2 : gset P) (Y : gset P), elem PRE X1 Y -> elem PRE (X1 ∪ X2) Y.
 Proof.
   apply tower; clear PRE.
   - intros P' HP ??????; eapply HP; eauto.
@@ -360,25 +385,35 @@ Proof.
     unfold copre_m, body.
     constructor.
     + intros q' hqq'; now apply CIH, h.(c_tau_).
-    + intros hp hq.
-      assert (hp_ : ∀ p : P, p ∈ X1 → p ⤓) by (intros ??; now apply hp, elem_of_union_l).
-      destruct (h.(c_now_) hp_ hq) as [ p [ p' [ pi [ hpp' out ] ] ]].
-      exists p, p'; split; eauto.
-      now apply elem_of_union_l.
+    + intros hp q' mem hq.
+      assert (hp_ : X1 ⤓).
+      { eapply termination_set_for_all. intros ??. 
+        eapply termination_if_termination_set_helper in hp;eauto.
+        now eapply elem_of_union_l. }
+      destruct (h.(c_now_) hp_ q' mem hq) as ( p & mem' & p' & pi & hpp' & out ).
+      exists p. split. 
+      * now eapply elem_of_union_l.
+      * exists p'; split; eauto.
     + intros μ q' ps' hp hqq' hps'.
-      destruct (wt_set_union _ _ _ hp hps') as [ ps1 [ ps2 [ h1 [ h2 -> ] ] ] ].
-      apply CIH.
+      assert (forall p, p ∈ X1 ∪ X2 -> p ⇓ [μ]) as hp'.
+      { intros; eapply convergence_forall_if_convergence_set; eauto. }
+      destruct (wt_set_union _ _ _ hp' hps') as (ps1 & ps2 & h1 & h2 & eq).
+      rewrite eq. apply CIH.
       eapply h.(c_step_); [ | exact hqq' | exact h1 ].
-      intros p i; now apply hp, elem_of_union_l.
+      eapply convergence_set_if_convergence_forall.
+      intros p i. eapply convergence_forall_if_convergence_set in hp;eauto. 
+      now eapply elem_of_union_l.
     + intros hp.
-      apply h.(c_cnv_).
-      intros p i; now apply hp, elem_of_union_l.
+      apply h.(c_cnv_). eapply termination_set_for_all.
+      intros p i. eapply termination_if_termination_set_helper in hp; eauto.
+      now eapply elem_of_union_l.
 Qed.
 
 Lemma coin_union_r `{@FiniteImagegLts P A H gLtsP}
-  `{PreAP : @PreExtAction P A H FinA PreA PreA_eq PreA_countable 𝝳 Φ gLtsP}
+  `{gLtsT : !gLtsEq T H}
+  `{AbsPT : @AbsAction P T FinA PreAct A H Φ 𝝳P _ _ }
   {PRE : Chain copre_m}
-  : forall (X1 X2 : gset P) (q : P), elem PRE X2 q -> elem PRE (X1 ∪ X2) q.
+  : forall (X1 X2 : gset P) (Y : gset P), elem PRE X2 Y -> elem PRE (X1 ∪ X2) Y.
 Proof.
   apply tower; clear PRE.
   - intros P' HP ??????; eapply HP; eauto.
@@ -386,33 +421,44 @@ Proof.
     unfold copre_m, body.
     constructor.
     + intros q' hqq'; now apply CIH, h.(c_tau_).
-    + intros hp hq.
-      assert (hp_ : ∀ p : P, p ∈ X2 → p ⤓) by (intros ??; now apply hp, elem_of_union_r).
-      destruct (h.(c_now_) hp_ hq) as [ p [ p' [ pi [ hpp' out ] ] ]].
-      exists p, p'; split; eauto.
-      now apply elem_of_union_r.
+    + intros hp q' mem hq.
+      assert (hp_ : X2 ⤓).
+      { eapply termination_set_for_all. intros ??. 
+        eapply termination_if_termination_set_helper in hp;eauto.
+        now eapply elem_of_union_r. }
+      destruct (h.(c_now_) hp_ q' mem hq) as (p & mem' & p' & pi & hpp' & out).
+      exists p. split.
+      * now apply elem_of_union_r.
+      * exists p'. repeat split; eauto.
     + intros μ q' ps' hp hqq' hps'.
-      destruct (wt_set_union _ _ _ hp hps') as [ ps1 [ ps2 [ h1 [ h2 -> ] ] ] ].
-      apply CIH.
+      assert (forall p, p ∈ X1 ∪ X2 -> p ⇓ [μ]) as hp'.
+      { intros; eapply convergence_forall_if_convergence_set; eauto. }
+      destruct (wt_set_union _ _ _ hp' hps') as (ps1 & ps2 & h1 & h2 & eq).
+      rewrite eq. apply CIH.
       eapply h.(c_step_); [ | exact hqq' | exact h2 ].
-      intros p i; now apply hp, elem_of_union_r.
+      eapply convergence_set_if_convergence_forall.
+      intros p i. eapply convergence_forall_if_convergence_set in hp;eauto.
+      now eapply elem_of_union_r.
     + intros hp.
-      apply h.(c_cnv_).
-      intros p i; now apply hp, elem_of_union_r.
+      apply h.(c_cnv_). eapply termination_set_for_all.
+      intros p i. eapply termination_if_termination_set_helper in hp; eauto.
+      now eapply elem_of_union_r.
 Qed.
 
 Lemma coin_elem_of `{@FiniteImagegLts P A H gLtsP}
-  `{PreAP : @PreExtAction P A H FinA PreA PreA_eq PreA_countable 𝝳 Φ gLtsP}
-  {PRE : Chain copre_m} (p : P) X: p ∈ X -> elem PRE X p.
+  `{gLtsT : !gLtsEq T H}
+  `{AbsPT : @AbsAction P T FinA PreAct A H Φ 𝝳P _ _ }
+  {PRE : Chain copre_m} (p : P) X: p ∈ X -> elem PRE X {[p]}.
 Proof.
-intro Hin. setoid_rewrite (union_difference_singleton_L p X Hin).
-apply coin_union_l, coin_refl.
+  intro Hin. setoid_rewrite (union_difference_singleton_L p X Hin).
+  apply coin_union_l, coin_refl.
 Qed.
 
 Lemma coin_choose `{@FiniteImagegLts P A H gLtsP}
-  `{PreAP : @PreExtAction P A H FinA PreA PreA_eq PreA_countable 𝝳 Φ gLtsP}
+  `{gLtsT : !gLtsEq T H}
+  `{AbsPT : @AbsAction P T FinA PreAct A H Φ 𝝳P _ _ }
   {PRE : Chain copre_m}
-  : forall {X : gset P} {q : P} {p : P}, p ∈ X -> elem PRE {[p]} q -> elem PRE X q.
+  : forall {X : gset P} {Y : gset P} {p : P}, p ∈ X -> elem PRE {[p]} Y -> elem PRE X Y.
 Proof.
   intros X q p Hin He.
   setoid_replace X with ({[p]} ∪ (X ∖ {[p]})) by now apply union_difference_singleton.
@@ -420,59 +466,72 @@ Proof.
 Qed.
 
 Lemma copre_fw_inv_l `{@FiniteImagegLts P A H gLtsP}
-  `{PreAP : @PreExtAction P A H FinA PreA PreA_eq PreA_countable 𝝳 Φ gLtsP}
+  `{gLtsT : !gLtsEq T H}
+  `{AbsPT : @AbsAction P T FinA PreAct A H Φ 𝝳P _ _ }
   `{@Prop_of_Inter P (mb A) A fw_inter H gLtsP MbgLts}
   {PRE : Chain (copre_m (P := P * mb A) (Q := P * mb A))} (p t: P):
   (∀ μ p', p ⟶{μ} p' <-> (p' = t /\ μ = τ)) ->
-  forall M (X : gset (P * mb A)) (q : P * mb A),
-    elem PRE ({[t ▷ M]} ∪ {[p ▷ M]} ∪ X) q
-    -> elem PRE ({[p ▷ M]} ∪ X) q.
+  forall M (X : gset (P * mb A)) (Y : gset (P * mb A)),
+    elem PRE ({[t ▷ M]} ∪ {[p ▷ M]} ∪ X) Y
+    -> elem PRE ({[p ▷ M]} ∪ X) Y.
 Proof.
   intros Hinv; apply tower; clear PRE.
   - intros P' HP ??????; eapply HP; eauto.
-  - intros PRE CIH M X q Hq.
+  - intros PRE CIH M X Y Hq.
     assert (Hpt : (p ▷ M) ⟶ (t ▷ M)) by (apply ParLeft, Hinv; tauto).
     constructor.
     + intros q' Hq'.
       apply CIH, Hq, Hq'.
-    + intros Ht Hs.
+    + intros Ht (p' , m') mem' Hs.
       destruct Hq as [ _ Hq _ _].
-      destruct Hq as (p1 & p2 & Hin & Hcnv & Hs' & Hout).
-      * intros p0 Hin. repeat rewrite elem_of_union in Hin.
+      edestruct Hq as (p1 & Hin & p2 & Hcnv & Hs' & Hout).
+      * eapply termination_set_for_all. intros p0 Hin. repeat rewrite elem_of_union in Hin.
         destruct Hin as [[Heqt | Heqp] | Hin].
         ++ apply elem_of_singleton_1 in Heqt. subst.
            apply terminate_preserved_by_lts_tau with (p ▷ M).
-           -- apply Ht. set_tac.
+           -- eapply termination_if_termination_set_helper in Ht; eauto.
+              set_tac.
            -- assumption.
         ++ apply elem_of_singleton_1 in Heqp. subst.
-           apply Ht. set_tac.
-        ++ apply Ht. set_tac.
+           eapply termination_if_termination_set_helper in Ht; eauto.
+           set_tac.
+        ++ eapply termination_if_termination_set_helper in Ht; eauto.
+           set_tac.
+      * exact mem'.
       * trivial.
       * repeat rewrite elem_of_union in Hin.
         destruct Hin as [[Heqt | Heqp] | Hin].
         ++ apply elem_of_singleton_1 in Heqt. subst.
-           exists (p ▷ M). exists p2. split; [ | split;[ | split ] ].
-           -- set_tac.
-           -- apply wt_tau with (t ▷ M); assumption.
-           -- apply Hs'.
-           -- eapply Hout.
+           exists (p ▷ M). split.
+           ** set_tac.
+           ** exists p2. split; [ | split]. 
+              -- apply wt_tau with (t ▷ M); assumption.
+              -- apply Hs'.
+              -- eapply Hout.
         ++ apply elem_of_singleton_1 in Heqp. subst.
-           exists (p ▷ M). exists p2. split; [ | split;[ | split ] ].
-           -- set_tac.
-           -- exact Hcnv.
-           -- exact Hs'.
-           -- exact Hout.
-        ++ exists p1. exists p2; intuition.
-           apply elem_of_union_r. set_tac.
-    + intros μ q' ps' Hμ1 Hμ2 Hwt. eapply Hq; [| eassumption |].
-      * intros p0 Hin. repeat rewrite elem_of_union in Hin.
+           exists (p ▷ M). split.
+           ** set_tac.
+           ** exists p2. split; [ | split].
+              -- exact Hcnv.
+              -- exact Hs'.
+              -- exact Hout.
+        ++ exists p1. split.
+           ** set_tac.
+           ** exists p2; intuition.
+    + intros μ qs' ps' Hμ1 Hμ2 Hwt. eapply Hq; [| eassumption |].
+      * eapply convergence_set_if_convergence_forall. intros p0 Hin.
+        repeat rewrite elem_of_union in Hin.
         destruct Hin as [[Heqt | Heqp] | Hin].
         ++ apply elem_of_singleton_1 in Heqt. subst.
            apply cnv_preserved_by_lts_tau with (p ▷ M).
-           -- apply Hμ1. set_tac.
+           -- eapply convergence_forall_if_convergence_set in Hμ1;eauto.
+              set_tac.
            -- assumption.
-        ++ apply elem_of_singleton_1 in Heqp. subst. apply Hμ1. set_tac.
-        ++ apply Hμ1. set_tac.
+        ++ apply elem_of_singleton_1 in Heqp. subst.
+           eapply convergence_forall_if_convergence_set in Hμ1;eauto.
+           set_tac.
+        ++ eapply convergence_forall_if_convergence_set in Hμ1;eauto.
+           set_tac.
       * destruct Hwt as [Hwt1 Hwt2].
         split.
         ++ intros p' Hp'. destruct (Hwt1 p' Hp') as [p0 [Hin Hp0]].
@@ -489,50 +548,62 @@ Proof.
            -- apply elem_of_singleton_1 in Heqp. subst.
               eapply Hwt2 with (p ▷ M); [set_tac|assumption].
            -- eapply Hwt2 with p'; [set_tac|]. apply Hμ.
-    + intros Ht. apply Hq. intros p0 Hin.
+    + intros Ht. apply Hq. eapply termination_set_for_all. intros p0 Hin.
       repeat rewrite elem_of_union in Hin. destruct Hin as [[Heqt | Heqp] | Hin].
       * apply elem_of_singleton_1 in Heqt. subst.
         apply terminate_preserved_by_lts_tau with (p ▷ M).
-        ++ apply Ht. set_tac.
+        ++ eapply termination_if_termination_set_helper in Ht;eauto. set_tac.
         ++ now apply Hpt.
       * apply elem_of_singleton_1 in Heqp. subst.
-        apply Ht. set_tac.
-      * apply Ht. set_tac.
+        eapply termination_if_termination_set_helper in Ht;eauto. set_tac.
+      * eapply termination_if_termination_set_helper in Ht;eauto. set_tac.
 Qed.
 
 Lemma copre_inv_l `{@FiniteImagegLts P A H gLtsP}
-  `{PreAP : @PreExtAction P A H FinA PreA PreA_eq PreA_countable 𝝳 Φ gLtsP}
-  {PRE : Chain copre_m} (p : P) X t q : (p ⟶ t) -> (forall μ p', p ⟹{μ} p' <-> t ⟹{μ} p') ->
-  elem PRE ({[t]} ∪ X) q -> elem PRE ({[p]} ∪ X) q.
+  `{gLtsT : !gLtsEq T H}
+  `{AbsPT : @AbsAction P T FinA PreAct A H Φ 𝝳P _ _ }
+  {PRE : Chain copre_m} (p : P) X t Y : (p ⟶ t) -> (forall μ p', p ⟹{μ} p' <-> t ⟹{μ} p') ->
+  elem PRE ({[t]} ∪ X) Y -> elem PRE ({[p]} ∪ X) Y.
 Proof.
-  intros Hpt Hinv; revert q.
+  intros Hpt Hinv; revert Y.
   apply tower; clear PRE.
   - intros P' HP ????; eapply HP; eauto.
-  - intros PRE CIH q h.
+  - intros PRE CIH Y h.
     constructor.
-    + intros q' Hq'.
+    + intros Y' HY'.
       now apply CIH, h.(c_tau_).
-    + intros Ht Hs.
-      destruct h.(c_now_) as [ p1 [ p' [ hp [ hpp' [ hp' ho ] ] ] ]]; eauto.
-      * intros p0 Hin.
+    + intros Ht p'' mem'' Hs.
+      edestruct h.(c_now_) as [ p1 [ hp [ p' [ hpp' [ hp' ho ] ] ] ]]; eauto.
+      * eapply termination_set_for_all. intros p0 Hin.
         apply elem_of_union in Hin; destruct Hin as [Heqt | Hin].
         -- apply elem_of_singleton_1 in Heqt; subst.
            apply terminate_preserved_by_lts_tau with p; eauto.
-           apply Ht; set_tac.
-        -- apply Ht; set_tac.
-      * apply elem_of_union in hp; destruct hp as [Heqt | Hin].
-        -- apply elem_of_singleton_1 in Heqt; subst.
-           exists p, p'; repeat split; [ set_tac | | | ]; trivial.
-           now apply wt_tau with t.
-        -- exists p1, p'; intuition.
-           now apply elem_of_union_r.
+           eapply termination_if_termination_set_helper in Ht;eauto. set_tac.
+        -- eapply termination_if_termination_set_helper in Ht;eauto. set_tac.
+      * apply elem_of_union in hp; destruct hp as [Heqt | Hin]. 
+        ++ exists p. split.
+           -- set_tac.
+           -- exists p'. apply elem_of_singleton_1 in Heqt; subst.
+              split; [ | split]. 
+              ** now apply wt_tau with t.
+              ** exact hp'.
+              ** exact ho.
+        ++ exists p1 ; intuition.
+           -- set_tac.
+           -- exists p'. split; [ | split]. 
+              ** exact hpp'.
+              ** exact hp'.
+              ** exact ho.
     + intros μ q' ps' hμ hqq' w.
       eapply h.(c_step_); eauto.
-      * intros p0 hin; apply elem_of_union in hin; destruct hin as [Heqt | Hin].
+      * eapply convergence_set_if_convergence_forall.
+        intros p0 hin; apply elem_of_union in hin; destruct hin as [Heqt | Hin].
         -- apply elem_of_singleton_1 in Heqt; subst.
            apply cnv_preserved_by_lts_tau with p; eauto.
-           apply hμ; set_tac.
-        -- apply hμ; set_tac.
+           eapply convergence_forall_if_convergence_set in hμ. exact hμ.
+           set_tac.
+        -- eapply convergence_forall_if_convergence_set in hμ. exact hμ.
+           set_tac.
       * destruct w as [Hwt1 Hwt2]; split.
         -- intros p' Hp'.
            destruct (Hwt1 p' Hp') as [p0 [Hin Hp0]].
@@ -546,15 +617,15 @@ Proof.
               eapply Hwt2 with p; [set_tac|]; apply Hinv, Hμ.
            ++ eapply Hwt2 with p'; [set_tac|]; apply Hμ.
     + intros Ht.
-      apply h.(c_cnv_); intros p0 Hin.
+      apply h.(c_cnv_); eapply termination_set_for_all; intros p0 Hin.
       apply elem_of_union in Hin; destruct Hin as [Heqt | Hin].
       * apply elem_of_singleton_1 in Heqt; subst.
         apply terminate_preserved_by_lts_tau with p; eauto.
-        apply Ht; set_tac.
-      * apply Ht; set_tac.
+        eapply termination_if_termination_set_helper in Ht;eauto. set_tac.
+      * eapply termination_if_termination_set_helper in Ht;eauto. set_tac.
 Qed.
 
-Global Instance copre_eq_rel_l `{@gLtsOba P A H gLtsEqP} `{!FiniteImagegLts P A}
+(* Global Instance copre_eq_rel_l `{@gLtsOba P A H gLtsEqP} `{!FiniteImagegLts P A}
   `{PreAP : @PreExtAction P A H FinA PreA PreA_eq PreA_countable 𝝳 Φ _}
   {PRE : Chain copre_m}: Proper ((eq_rel_set) ==> (=) ==> (impl)) (elem PRE).
 Proof.
@@ -574,7 +645,7 @@ Proof.
         exists p''; exists r; repeat split; trivial; now rewrite Heqr.
     + intros μ q' ps' hμ hqq' w.
       apply (wt_set_from_pset_spec_eq_rel_set (symmetry hXX')) in w
-        as (ps'' & Heqps' & HXps''); [|trivial].
+        as (X'' & Heqps' & HXps''); [|trivial].
       apply CIH with ps''; [now symmetry|].
       eapply h.(c_step_); eauto.
       intros p Hp. apply hXX' in Hp as (p'' & Hin & Heqp'').
@@ -583,5 +654,4 @@ Proof.
       apply h.(c_cnv_); intros p0 Hin.
       apply hXX' in Hin as (p'' & Hin & Heqp'').
       eapply terminate_preserved_by_eq2; [apply symmetry, Heqp''|auto with *].
-Qed.
-*)
+Qed. *)
